Revert CompCertX program holes
In CertiKOS we make sure the programs follow a predetermined structure so that
the resulting global environments have a fixed symbol -> block mapping. To make
that possible, in CompCertX we allow empty declarations in programs.

Instead, for Composable Compcert the plan is to use the linking infrastructure
to add external declarations as needed, so we can drop the corresponding
changes to Compcert. This commit may be incomplete as not every pass builds at
the moment.

backend/ValueAnalysis.v
@@ -220,13 +220,11 @@ Definition definitive_initializer (init: list init_data) : bool :=
   | _ => true
   end.
 
-Definition alloc_global (rm: romem) (idg: ident * option (globdef fundef unit)): romem :=
+Definition alloc_global (rm: romem) (idg: ident * globdef fundef unit): romem :=
   match idg with
-  | (id, None) =>
+  | (id, Gfun f) =>
       PTree.remove id rm
-  | (id, Some (Gfun f)) =>
-      PTree.remove id rm
-  | (id, Some (Gvar v)) =>
+  | (id, Gvar v) =>
       if v.(gvar_readonly) && negb v.(gvar_volatile) && definitive_initializer v.(gvar_init)
       then PTree.set id (store_init_data_list (ablock_init Pbot) 0 v.(gvar_init)) rm
       else PTree.remove id rm
@@ -1765,7 +1763,7 @@ Lemma alloc_global_match:
   Genv.alloc_global ge m idg = Some m' ->
   initial_mem_match bc m' (Genv.add_global g idg).
 Proof.
-  intros; red; intros. destruct idg as [id1 [[fd | gv]|]]; simpl in *.
+  intros; red; intros. destruct idg as [id1 [fd | gv]]; simpl in *.
 - destruct (Mem.alloc m 0 1) as [m1 b1] eqn:ALLOC.
   unfold Genv.find_symbol in H2; simpl in H2.
   unfold Genv.find_var_info, Genv.find_def in H3; simpl in H3.
@@ -1862,13 +1860,9 @@ Definition romem_consistent (defmap: PTree.t (globdef fundef unit)) (rm: romem) 
 Lemma alloc_global_consistent:
   forall dm rm idg,
   romem_consistent dm rm ->
-  romem_consistent (match snd idg with
-                      | Some g => PTree.set (fst idg) g dm
-                      | None => PTree.remove (fst idg) dm
-                    end)
-                   (alloc_global rm idg).
+  romem_consistent (PTree.set (fst idg) (snd idg) dm) (alloc_global rm idg).
 Proof.
-  intros; red; intros. destruct idg as [id1 [[f1 | v1] | ]]; simpl in *.
+  intros; red; intros. destruct idg as [id1 [f1 | v1]]; simpl in *.
 - rewrite PTree.grspec in H0. destruct (PTree.elt_eq id id1); try discriminate.
   rewrite PTree.gso by auto. apply H; auto.
 - destruct (gvar_readonly v1 && negb (gvar_volatile v1) && definitive_initializer (gvar_init v1)) eqn:RO.
@@ -1878,21 +1872,14 @@ Proof.
 * apply H; auto.
 + rewrite PTree.grspec in H0. destruct (PTree.elt_eq id id1); try discriminate.
   rewrite PTree.gso by auto. apply H; auto.
-- rewrite ! PTree.grspec in * |- *.
-  destruct (PTree.elt_eq id id1); try discriminate.
-  eauto.
 Qed.
 
 Lemma romem_for_consistent:
-  forall cunit, romem_consistent (prog_defmap cunit) (romem_for_wp cunit).
+  forall cunit, romem_consistent (prog_defmap cunit) (romem_for cunit).
 Proof.
   assert (REC: forall l dm rm,
             romem_consistent dm rm ->
-            romem_consistent (fold_left (fun m idg =>
-                                           match snd idg with
-                                             | Some g => PTree.set (fst idg) g m
-                                             | None => PTree.remove (fst idg) m
-                                           end) l dm)
+            romem_consistent (fold_left (fun m idg => PTree.set (fst idg) (snd idg) m) l dm)
                              (fold_left alloc_global l rm)).
   { induction l; intros; simpl; auto. apply IHl. apply alloc_global_consistent; auto. }
   intros. apply REC.
